coq/DNNRC/Typing/TOpsInferSub.v
@@ -146,6 +146,12 @@ Section TOpsInferSub.
       | ADistinct =>
         let τ₁' := τ₁ ⊔ (Coll ⊥) in
         lift (fun τ => (Coll τ, τ₁')) (tuncoll τ₁')
+      | AOrderBy sl =>
+        let τ₁' := τ₁ ⊔ (Coll ⊥) in
+        match (tunrecproject (List.map fst sl) τ₁') with
+        | Some _ => Some (τ₁, τ₁')
+        | None => None
+        end
       | ARec s => Some (Rec Closed ((s, τ₁)::nil) eq_refl, τ₁)
         (* Note that ⊥ does not get further constrained by these *)
       | ADot s =>
